add delete spec & commutativity

LeanYjs/Algorithm/Delete/Basic.lean
@@ -2,80 +2,28 @@ import LeanYjs.Item
 import LeanYjs.Algorithm.Invariant.Basic
 import LeanYjs.Algorithm.Invariant.YjsArray
 
+mutual
+def deleteItemById (item : YjsItem A) (id : YjsId) : YjsItem A :=
+  match item with
+  | YjsItem.mk o r iid c d =>
+    if iid = id then
+      YjsItem.mk (deletePtrById o id) (deletePtrById r id) iid c true
+    else
+      YjsItem.mk (deletePtrById o id) (deletePtrById r id) iid c d
+
+def deletePtrById (ptr : YjsPtr A) (id : YjsId) : YjsPtr A :=
+  match ptr with
+  | YjsPtr.itemPtr item => YjsPtr.itemPtr (deleteItemById item id)
+  | YjsPtr.first => YjsPtr.first
+  | YjsPtr.last => YjsPtr.last
+end
+
+/--
+  Delete the item with the given id from the array by marking it as deleted.
+  Not only the item itself but also all its origins and right origins are marked as deleted.
+  This is done to maintain the invariants of the Yjs array.
+  In real Yjs implementation, it just change the field and does not traverse the origins because the origin/rightOrigins are references to other items.
+-/
 def deleteById (arr : Array (YjsItem A)) (id : YjsId) : Array (YjsItem A) :=
   -- Mark the item with the given id as deleted
-  arr.map (fun item =>
-    if item.id = id then
-      YjsItem.mk item.origin item.rightOrigin item.id item.content true
-    else
-      item)
-
-theorem deleteById_mem_iff (arr : Array (YjsItem A)) (id : YjsId) x :
-  x ∈ deleteById arr id ↔
-    (x.id = id ∧ x.deleted = true ∧ ∃d, {x with deleted := d } ∈ arr) ∨
-    (x.id ≠ id ∧ x ∈ arr) := by
-  constructor
-  . intro hmem
-    simp [deleteById] at hmem
-    obtain ⟨ a, ha, heq ⟩ := hmem
-    split at heq
-    . left
-      obtain ⟨ _, _, _, _, d ⟩ := a
-      simp at *
-      subst x; simp
-      constructor
-      . assumption
-      . cases d with
-        | true => right; assumption
-        | false => left; assumption
-    . right
-      subst heq
-      constructor <;> assumption
-  . intros hor
-    simp [deleteById]
-    cases hor with
-    | inl h =>
-      obtain ⟨ hid, hdeleted, d, hmem ⟩ := h
-      use { origin := x.origin, rightOrigin := x.rightOrigin, id := x.id, content := x.content, deleted := d }
-      constructor; assumption
-      simp
-      subst id; simp
-      obtain ⟨ _, _, _, _, _ ⟩ := x
-      simp at *
-      assumption
-    | inr h =>
-      obtain ⟨ hid, hx ⟩ := h
-      use x
-      constructor; assumption
-      simp
-      intros; contradiction
-
--- theorem YjsArrInvariant_deleteById (arr : Array (YjsItem A)) (id : YjsId) :
---   YjsArrInvariant arr.toList ->
---   YjsArrInvariant (deleteById arr id).toList := by
---   intro hinv
---   constructor
---   . constructor
---     . simp [ArrSet]
---     . simp [ArrSet]
---     . intros o r cid c d ha
---       simp [ArrSet] at ha
---       rw [deleteById_mem_iff] at ha; simp at ha
---       obtain ⟨ hcid, hd, ha ⟩ := ha
---       cases ha with
---       | inl h =>
---         have h : ArrSet arr.toList <| YjsPtr.itemPtr { origin := o, rightOrigin := r, id := cid, content := c, deleted := false } := by
---           simp [ArrSet]; assumption
---         apply hinv.closed.closedLeft at h
---         rcases o with ⟨ o ⟩ | _ | _ <;> simp [ArrSet] at *
---         rw [deleteById_mem_iff]
---       replace ⟨ a, hmem, ha ⟩ := ha
---       obtain ⟨ ao, ar, aid, ac, ad ⟩ := a; simp at *
---       have ha' := hinv.closed.closedLeft o r id c (a.id = id)
---       split at ha <;> simp [ArrSet] at *
---       rcases o with ⟨ o ⟩ | _ | _ <;> simp at *
---       use { o with deleted := o.id = id }; simp
-
-theorem deleteById_commutative (arr : Array (YjsItem A)) (id1 id2 : YjsId) :
-  deleteById (deleteById arr id1) id2 = deleteById (deleteById arr id2) id1 := by
-  grind only [deleteById, = Array.size_map, = Array.getElem_map]
+  arr.map fun item => deleteItemById item id
