LeanYjs/Algorithm/Delete/Commutative.lean
@@ -1,0 +1,78 @@
+import LeanYjs.Algorithm.Delete.Basic
+
+theorem deleteItemById_deletePtrById_commutative {id1 id2 : YjsId} :
+  (∀item : YjsItem A, item.size = n → deleteItemById (deleteItemById item id1) id2 = deleteItemById (deleteItemById item id2) id1) ∧
+  (∀ptr : YjsPtr A, ptr.size = n → deletePtrById (deletePtrById ptr id1) id2 = deletePtrById (deletePtrById ptr id2) id1) := by
+  apply Nat.strongRec' (p := fun n =>
+      (∀item, item.size = n → deleteItemById (deleteItemById item id1) id2 = deleteItemById (deleteItemById item id2) id1) ∧
+      (∀ptr, ptr.size = n → deletePtrById (deletePtrById ptr id1) id2 = deletePtrById (deletePtrById ptr id2) id1))
+  intros n ih
+  constructor
+  . intros item hsize
+    obtain ⟨ o, r, id, c, d ⟩ := item
+    simp [YjsItem.size] at hsize
+    simp [deleteItemById]
+    by_cases h_id1 : (id = id1)
+    . subst id; simp
+      by_cases h_id2 : (id1 = id2)
+      . subst id1; simp
+      . split; contradiction
+        simp [deleteItemById]
+        have ⟨ _, h_o ⟩ := ih o.size (by omega)
+        replace h_o := h_o o rfl
+        have ⟨ _, h_r ⟩ := ih r.size (by omega)
+        replace h_r := h_r r rfl
+        constructor <;> assumption
+    . by_cases h_id2 : (id = id2)
+      . subst id; simp
+        split; contradiction
+        simp [deleteItemById]
+        have ⟨ _, h_o ⟩ := ih o.size (by omega)
+        replace h_o := h_o o rfl
+        have ⟨ _, h_r ⟩ := ih r.size (by omega)
+        replace h_r := h_r r rfl
+        constructor <;> assumption
+      . split; contradiction
+        simp [deleteItemById]
+        split; contradiction
+        simp
+        have ⟨ _, h_o ⟩ := ih o.size (by omega)
+        replace h_o := h_o o rfl
+        have ⟨ _, h_r ⟩ := ih r.size (by omega)
+        replace h_r := h_r r rfl
+        constructor <;> assumption
+  . intros p h_size
+    cases p with
+    | first => simp [deletePtrById]
+    | last => simp [deletePtrById]
+    | itemPtr item =>
+      simp [YjsPtr.size] at h_size
+      simp [deletePtrById]
+      have ⟨ h_item, _ ⟩ := ih item.size (by omega)
+      replace h_item := h_item item rfl
+      assumption
+
+theorem deleteItemById_commutative (item : YjsItem A) (id1 id2 : YjsId) :
+  deleteItemById (deleteItemById item id1) id2 = deleteItemById (deleteItemById item id2) id1 := by
+  have ⟨ h_item, _ ⟩ := deleteItemById_deletePtrById_commutative (A := A) (n := item.size) (id1 := id1) (id2 := id2)
+  apply h_item item rfl
+
+theorem deletePtrById_commutative (ptr : YjsPtr A) (id1 id2 : YjsId) :
+  deletePtrById (deletePtrById ptr id1) id2 = deletePtrById (deletePtrById ptr id2) id1 := by
+  have ⟨ _, h_ptr ⟩ := deleteItemById_deletePtrById_commutative (A := A) (n := ptr.size) (id1 := id1) (id2 := id2)
+  apply h_ptr ptr rfl
+
+theorem deleteItemById_id (item : YjsItem A) (id : YjsId) :
+  (deleteItemById item id).id = item.id := by
+  obtain ⟨ o, r, iid, c, d ⟩ := item
+  simp [deleteItemById]
+  grind only
+
+theorem deleteById_commutative (arr : Array (YjsItem A)) (id1 id2 : YjsId) :
+  deleteById (deleteById arr id1) id2 = deleteById (deleteById arr id2) id1 := by
+  apply Array.ext
+  . simp [deleteById]
+  . intro i hi₁ hi₂
+    simp [deleteById] at hi₁ hi₂
+    simp [deleteById]
+    apply deleteItemById_commutative
